<?xml version="1.0" encoding="UTF-8" ?>

<!-- <subsection xmlns:xi="http://www.w3.org/2001/XInclude" xml:id="subsec-name-dc"> 
    <title>Participate</title> -->
    
    <worksheet xml:id="ws-matrixmultiplication" margin="1in" bottom="1.25cm"><title component="print-worksheets">Participate: Matrix Multiplication</title><title component="online-worksheets">Participate</title>
      <objectives>
        <ul>
          <li>
            <p>
              Be able to perform matrix multiplication when it is possible.
            </p>
          </li>
          <li>
            <p>
              Explore ways in which matrix multiplication acts like multiplication of numbers, and 
              ways in which matrix multiplication is different.  
            </p>
          </li>
        </ul>
</objectives>
      <!-- <introduction>
        <p>
          something else to say?
        </p>
      </introduction> -->
      <page>
        <!-- Still need something about the identity matrix, and maybe (a+b)^2 \neq a^2+2ab+b^2 -->
        <activity>
      <statement>
      <p> Consider the matrices
	<me>
	  A = \left[\begin{array}{rrr}
	  1 \amp 3 \amp 2 \\
	  -3 \amp 4 \amp -1 \\
	  \end{array}\right],~~~
	  B = \left[\begin{array}{rr}
	  3 \amp 0 \\
	  1 \amp 2 \\
	  -2 \amp -1 \\
	  \end{array}\right]
	</me>.
	<ol marker="a.">
	  <li>
	    <p>
	      Before
	      computing, first explain why the shapes of
	      <m>A</m> and <m>B</m> enable us to form the product <m>AB</m>.
	      Then describe the shape of <m>AB</m>.
	    </p>
	  </li>

	  <li><p> Compute the product <m>AB</m>. </p></li>

	  <li><p> Sage can multiply matrices using the <c>*</c>
	  operator.  Define the matrices <m>A</m> and <m>B</m> in the
	  Sage cell below and
	  check your work by computing <m>AB</m>.
	  <sage>
	    <input>
	    </input>
	  </sage>
	  </p></li>
	  
	  <li><p> Are we able to form the matrix product <m>BA</m>?  If
	  so, use the Sage cell above to find <m>BA</m>.  Is it
	  generally true that <m>AB = BA</m>?
	  </p></li>
	  
	  <li><p> Suppose we form the three matrices.
	  <me>
	    A = \left[\begin{array}{rr}
	    1 \amp 2 \\
	    3 \amp -2 \\
	    \end{array}\right],
	    B = \left[\begin{array}{rr}
	    0 \amp 4 \\
	    2 \amp -1 \\
	    \end{array}\right],
	    C = \left[\begin{array}{rr}
	    -1 \amp 3 \\
	    4 \amp 3 \\
	    \end{array}\right]
	    </me>.
	    Compare what happens when you compute <m>A(B+C)</m> and <m>AB
	    + AC</m>.  State your finding as a general principle.
	    <sage>
	      <input>
	      </input>
	    </sage>
	    
	  </p></li>
	  
	  <li><p> Compare the results of evaluating <m>A(BC)</m> and
	  <m>(AB)C</m> and state your finding as a general
	  principle. </p></li> 
	  
	  <li><p> When we are dealing with real numbers, we know if
	  <m>a\neq 0</m> and <m>ab = ac</m>, then <m>b=c</m>.  Define
	  matrices 
	  <me>
	    A = \left[\begin{array}{rr}
	    1 \amp 2 \\
	    -2 \amp -4 \\
	    \end{array}\right],
	    B = \left[\begin{array}{rr}
	    3 \amp 0 \\
	    1 \amp 3 \\
	    \end{array}\right],
	    C = \left[\begin{array}{rr}
	    1 \amp 2 \\
	    2 \amp 2 \\
	    \end{array}\right]
	  </me>
	  and compute <m>AB</m> and <m>AC</m>.
	  <sage>
	    <input>
	    </input>
	  </sage>
	  If <m>AB = AC</m>, is it necessarily true that <m>B = C</m>?
	  </p></li>
	  
	  <li><p> Again, with real numbers, we know that if <m>ab =
	  0</m>, then either <m>a = 0</m> or <m>b=0</m>.  Define
	  <me>
	    A = \left[\begin{array}{rr}
	    1 \amp 2 \\
	    -2 \amp -4 \\
	    \end{array}\right],
	    B = \left[\begin{array}{rr}
	    2 \amp -4 \\
	    -1 \amp 2 \\
	    \end{array}\right]
	  </me>
	  and compute <m>AB</m>.
	  <sage>
	    <input>
	    </input>
	  </sage>
	  If <m>AB = 0</m>, is it necessarily true that either
	  <m>A=0</m> or <m>B=0</m>?
	  </p></li>
	</ol>
      </p>
      </statement>
      
      <solution>
	<p><ol marker="a.">
	  <li><p>
	    The product <m>AB</m> exists because the number of columns
	    of <m>A</m> equals the number of rows of <m>B</m>.  The
	    dimensions of <m>AB</m> are <m>2\times 2</m>.
	  </p></li>

	  <li><p>
	    We have
	    <m>AB =
	    \left[\begin{array}{rr}
	    2 \amp 4 \\
	    -3 \amp 9
	    \end{array}\right]
	    </m>.
	  </p></li>

	  <li><p> Define
	    <cd>
A = matrix(2, 3, [1, 3, 2, -3, 4, -1])
B = matrix(3, 2, [3, 0, 1, 2, -2, -1])
A*B
	    </cd>
	  </p></li>

	  <li><p>
	    Yes, we can form the product <m>BA</m> because the number
	    of columns of <m>B</m> equals the number of rows of
	    <m>A</m>.  This product <m>AB</m> will be <m>3\times3</m>,
	    however, so it must be true that <m>AB\neq BA</m>.
	  </p></li>

	  <li><p> We find that <m>A(B+C)=AB + AC</m>.
	  </p></li>

	  <li><p> We find that <m>A(BC) = (AB)C</m>.
	  </p></li>

	  <li><p>
	    It is not generally true that <m>B=C</m> if <m>AB=AC</m>,
	    as illustrated by this example.
	  </p></li>

	  <li><p>
	    It is not generally true that <m>A=0</m> or <m>B=0</m> if
	    <m>AB=0</m>, as illustrated by this example.
	  </p></li>

	</ol></p>
      </solution>

      <answer>
	<p><ol marker="a.">
	  <li><p>
	    The product <m>AB</m> exists because the number of columns
	    of <m>A</m> equals the number of rows of <m>B</m>.  The
	    dimensions of <m>AB</m> are <m>2\times 2</m>.
	  </p></li>

	  <li><p>
	    We have
	    <m>AB =
	    \left[\begin{array}{rr}
	    2 \amp 4 \\
	    -3 \amp 9
	    \end{array}\right]
	    </m>.
	  </p></li>

	  <li><p> Define
	    <cd>
A = matrix(2, 3, [1, 3, 2, -3, 4, -1])
B = matrix(3, 2, [3, 0, 1, 2, -2, -1])
A*B
	    </cd>
	  </p></li>

	  <li><p>
	    It is not generally true that <m>AB=BA</m>.
	  </p></li>

	  <li><p> We find that <m>A(B+C)=AB + AC</m>.
	  </p></li>

	  <li><p> We find that <m>A(BC) = (AB)C</m>.
	  </p></li>

	  <li><p>
	    It is not generally true that <m>B=C</m> if <m>AB=AC</m>.
	  </p></li>

	  <li><p>
	    It is not generally true that <m>A=0</m> or <m>B=0</m> if
	    <m>AB=0</m>.
	  </p></li>

	</ol></p>
      </answer>

      
    </activity>

      
      </page>
    </worksheet>
    <!-- </subsection> -->